boogie_examples/all_exists/Hypa/refine.bpl
@@ -21,7 +21,6 @@
 //     }
 // }
 
-
 // [exists]
 // int x;
 // int c;
@@ -34,7 +33,6 @@
 //     while (time > 0) {
 //         time = time - 1;
 //         x = x + 1;
-//         x = x + 1;
 //     }
 // } else {
 //     x = 0;
@@ -42,7 +40,7 @@
 //     while (time > 0) {
 //         time = time - 1;
 //         s = *;
-//         x = x + s + 1;
+//         x = x + s;
 //     }
 // }
 
@@ -52,16 +50,17 @@
 // [post]
 // (c_0 == 0) => (c_1 == 1 && x_0 == x_1)
 
-// verifies.
+
+// Verifies.
 
 procedure example (time1: int, time2: int) returns (c1: int, c2: int, x1: int, x2: int)
     requires (time1 == time2);
-    // requires (time1 >= 0);  // added
     ensures (c1 == 0 ==> (c2 == 1 && x1 == x2));
 {
     var k1: int; var k2: int;
     var s1: int;  var s2: int;
     var b1: bool; var b2: bool;
+    var vsnap: int;
     k1 := time1; k2 := time2;
 
     havoc b1;
@@ -82,41 +81,53 @@ procedure example (time1: int, time2: int) returns (c1: int, c2: int, x1: int, x
         x1 := 0;
         c1 := 1;
         while (k1 > 0)
+        invariant ((time1 <= 0 ==> x1 == 0));
+        invariant (time1 >= k1);
         {
             k1 := k1 - 1;
             havoc s1;
             x1 := x1 + s1;
+
         }
     }
+
+
     assert (exists v:bool :: v != b1); // added by chk
     havoc b2;
     assume (b2 != b1);
-    
+
     if (b2)
     {
         x2 := 0;
         c2 := 0;
         while (k2 > 0)
         {
+            vsnap := k2; // variant k2
+
             k2 := k2 - 1;
             x2 := x2 + 1;
-            x2 := x2 + 1;
 
+            assert (0 <= k2 && k2 < vsnap); // variant decreases
         }
     } else
     {
         x2 := 0;
         c2 := 1;
+
         while (k2 > 0)
            invariant (x2 + k2 == time2);
            invariant (time2 <= 0 ==> x2 == 0);
            invariant (time2 > 0 ==> k2 >= 0);
         {
+            vsnap := k2; // variant k2
+
             k2 := k2 - 1;
-            assert (exists v:int :: v == 0); // added by chk 
+            assert (exists v:int :: v == 1); // added by chk 
             havoc s2;
-            assume s2 == 0;
-            x2 := x2 + s2 + 1;
+            assume s2 == 1;
+            x2 := x2 + s2;
+
+            assert (0 <= k2 && k2 < vsnap); // variant decreases
         }
     }
 
